Major clean up of Ctxs

theories/Context.v
@@ -29,531 +29,15 @@
 From Coq Require Import
      NArith.BinNat
      Bool.Bool
-     Init.Datatypes
-     Init.Decimal
-     Logic.EqdepFacts
      Numbers.DecimalString
      Strings.Ascii
      Strings.String.
 
 From Equations Require Import Equations.
-From stdpp Require
-     base.
 From Katamaran Require Import
      Notation Prelude.
 
-Set Implicit Arguments.
-
-(* Type of contexts. This is a list of bindings of type B. This type and
-   subsequent types use the common notation of snoc lists. *)
-Inductive Ctx (B : Set) : Set :=
-| ctx_nil
-| ctx_snoc (Γ : Ctx B) (b : B).
-
-Section TransparentObligations.
-  Local Set Transparent Obligations.
-  Derive NoConfusion for Ctx.
-End TransparentObligations.
-
-Arguments ctx_nil {_}.
-Arguments ctx_snoc {_} _%ctx _%ctx.
-Bind Scope ctx_scope with Ctx.
-
-Section WithBinding.
-  Context {B : Set}.
-
-  Global Instance ctx_eqdec {eqB : EqDec B} : EqDec (Ctx B) :=
-    fix ctx_eqdec (Γ Δ : Ctx B) {struct Γ} : dec_eq Γ Δ :=
-      match Γ , Δ with
-      | ctx_nil      , ctx_nil      => left eq_refl
-      | ctx_snoc Γ b , ctx_snoc Δ c => f_equal2_dec ctx_snoc noConfusion_inv
-                                                    (ctx_eqdec Γ Δ) (eq_dec b c)
-      | _            , _            => right noConfusion_inv
-      end.
-
-  Fixpoint ctx_lookup (Γ : Ctx B) (n : nat) : option B :=
-    match Γ , n with
-    | ctx_snoc _ b , O   => Some b
-    | ctx_snoc Γ _ , S n => ctx_lookup Γ n
-    | _            , _   => None
-    end.
-
-  (* Concatenation of two contexts. *)
-  Fixpoint ctx_cat (Γ1 Γ2 : Ctx B) {struct Γ2} : Ctx B :=
-    match Γ2 with
-    | ctx_nil       => Γ1
-    | ctx_snoc Γ2 τ => ctx_snoc (ctx_cat Γ1 Γ2) τ
-    end.
-
-  (* This is a predicate that that encodes that the de Bruijn index n points
-     to the binding b in Γ. *)
-  Fixpoint ctx_nth_is (Γ : Ctx B) (n : nat) (b : B) {struct Γ} : Prop :=
-    match Γ , n with
-    | ctx_snoc _ x , O   => x = b
-    | ctx_snoc Γ _ , S n => ctx_nth_is Γ n b
-    | _            , _   => False
-    end.
-
-  Lemma ctx_nth_is_right_exact {Γ : Ctx B} (n : nat) (b1 b2 : B) :
-    ctx_nth_is Γ n b1 -> ctx_nth_is Γ n b2 -> b1 = b2.
-  Proof.
-    revert n.
-    induction Γ.
-    - intros ? [].
-    - cbn in *.
-      destruct n eqn:E.
-      + congruence.
-      + apply IHΓ.
-  Qed.
-
-  Section WithUIP.
-
-    Context {UIP_B : UIP B}.
-
-    Fixpoint ctx_nth_is_proof_irrelevance {Γ : Ctx B} (n : nat) (b : B) {struct Γ} :
-      forall (p q : ctx_nth_is Γ n b), p = q.
-    Proof.
-      destruct Γ; intros p q.
-      - destruct q.
-      - destruct n; cbn in *.
-        + apply uip.
-        + apply (ctx_nth_is_proof_irrelevance _ n _ p q).
-    Defined.
-
-    Global Instance eqdec_ctx_nth {Γ n b} : EqDec (ctx_nth_is Γ n b).
-    Proof. intros p q. left. apply ctx_nth_is_proof_irrelevance. Defined.
-
-    Lemma ctx_nth_is_proof_irrelevance_refl {Γ : Ctx B} (n : nat) (b : B) (p : ctx_nth_is Γ n b) :
-      ctx_nth_is_proof_irrelevance n b p p = eq_refl.
-    Proof. apply uip. Qed.
-
-  End WithUIP.
-
-  Section InCtx.
-    (* Set locally only for the definition of InCtx. *)
-    Local Set Primitive Projections.
-
-     (* InCtx represents context containment proofs. This is essentially a
-        well-typed de Bruijn index, i.e. a de Bruijn index with a proof that it
-        resolves to the binding b. This record type is defined using primitive
-        projections to get eta-conversion definitionally. *)
-    Class InCtx (b : B) (Γ : Ctx B) : Set :=
-      MkInCtx
-        { inctx_at: nat;
-          inctx_valid: ctx_nth_is Γ inctx_at b
-        }.
-
-    Global Arguments MkInCtx [_ _] _ _.
-    Global Arguments inctx_at [_ _] _.
-    Global Arguments inctx_valid [_ _] _.
-
-    Global Program Instance NoConfusionPackage_InCtx {uip_B : UIP B} {b Γ} : NoConfusionPackage (InCtx b Γ) :=
-       {| NoConfusion xIn yIn := NoConfusion (inctx_at xIn) (inctx_at yIn);
-          noConfusion xIn yIn (e : NoConfusion (inctx_at xIn) (inctx_at yIn)) :=
-            match noConfusion e in _ = y
-              return forall q, xIn = {| inctx_at := y; inctx_valid := q |}
-            with
-            | eq_refl => fun q => f_equal (MkInCtx _) (ctx_nth_is_proof_irrelevance _ _ (inctx_valid xIn) q)
-            end (inctx_valid yIn);
-          noConfusion_inv (xIn yIn : InCtx b Γ) (e : xIn = yIn) :=
-            noConfusion_inv (f_equal (@inctx_at b Γ) e);
-       |}.
-    Next Obligation.
-      intros ? ? ? [m p] [n q] e. cbn [inctx_at] in *.
-      change (NoConfusion _ _) with (NoConfusion m n) in e.
-      destruct (noConfusion e) eqn:?. cbn.
-      destruct (ctx_nth_is_proof_irrelevance m b p q). cbn.
-      destruct m.
-      - destruct e. reflexivity.
-      - apply uip.
-    Qed.
-    Next Obligation.
-      intros ? ? ? [m p] [n q] e; intros.
-      destruct e.
-      destruct Γ; cbn in *. contradiction.
-      destruct m, n.
-      - destruct p. cbn. now rewrite EqDec.uip_refl_refl.
-      - destruct p. cbn. now rewrite EqDec.uip_refl_refl.
-      - cbn. rewrite ctx_nth_is_proof_irrelevance_refl. reflexivity.
-      - cbn. rewrite ctx_nth_is_proof_irrelevance_refl. reflexivity.
-    Qed.
-
-  End InCtx.
-
-  (* Two proofs of context containment are equal of the deBruijn indices are equal *)
-  Definition InCtx_eqb {Γ} {b1 b2 : B}
-             (b1inΓ : InCtx b1 Γ)
-             (b2inΓ : InCtx b2 Γ) : bool :=
-    Nat.eqb (inctx_at b1inΓ) (inctx_at b2inΓ).
-
-  Lemma InCtx_eqb_spec `{UIP B} {Γ} {b1 b2 : B} (b1inΓ : InCtx b1 Γ) (b2inΓ : InCtx b2 Γ) :
-    reflect
-      (existT _ b1inΓ = existT _ b2inΓ :> sigT (fun b => InCtx b Γ))
-      (InCtx_eqb b1inΓ b2inΓ).
-  Proof.
-    destruct b1inΓ as [m p], b2inΓ as [n q]; cbn.
-    destruct (NPeano.Nat.eqb_spec m n); constructor.
-    - subst. pose proof (ctx_nth_is_right_exact _ _ _ p q). subst.
-      f_equal. f_equal. apply ctx_nth_is_proof_irrelevance.
-    - intros e. depelim e. destruct n, m; cbn in H0; congruence.
-  Qed.
-
-  (* These are *constructors* for InCtx. *)
-  Definition inctx_zero {b : B} {Γ : Ctx B} : InCtx b (ctx_snoc Γ b) :=
-    @MkInCtx _ (ctx_snoc Γ b) 0 eq_refl.
-  Definition inctx_succ {b : B} {Γ : Ctx B} {b' : B} (bIn : InCtx b Γ) :
-    InCtx b (ctx_snoc Γ b') :=
-    @MkInCtx _ (ctx_snoc Γ b') (S (inctx_at bIn)) (inctx_valid bIn).
-
-  Inductive NilView {b : B} (i : InCtx b ctx_nil) : Set :=.
-
-  Definition nilView {b : B} (i : InCtx b ctx_nil) : NilView i :=
-    match inctx_valid i with end.
-
-  Inductive SnocView (Γ : Ctx B) {b' : B} : forall b, InCtx b (ctx_snoc Γ b') -> Set :=
-  | snocViewZero                     : SnocView inctx_zero
-  | snocViewSucc {b} (i : InCtx b Γ) : SnocView (inctx_succ i).
-  Global Arguments snocViewZero {_ _}.
-
-  Definition snocView {Γ} {b b' : B} (i : InCtx b (ctx_snoc Γ b')) :
-    @SnocView Γ b' b i :=
-    match inctx_at i as n return forall p, SnocView (MkInCtx n p)
-    with
-    | O   => fun p => match p with eq_refl => snocViewZero end
-    | S n => fun p => snocViewSucc (MkInCtx n p)
-    end (inctx_valid i).
-
-  Inductive InCtxView {b : B} : forall Γ, InCtx b Γ -> Set :=
-  | inctxViewZero {Γ}                    : @InCtxView b (ctx_snoc Γ b) inctx_zero
-  | inctxViewSucc {Γ b'} (i : InCtx b Γ) : @InCtxView b (ctx_snoc Γ b') (inctx_succ i).
-
-  Definition inctxView {b Γ} (bIn : InCtx b Γ) : InCtxView bIn.
-  Proof.
-    destruct Γ.
-    - destruct (nilView bIn).
-    - destruct (snocView bIn); constructor.
-  Defined.
-
-  Fixpoint inctx_cat_left {b : B} {Γ : Ctx B} (Δ : Ctx B) (bIn : InCtx b Γ) : InCtx b (ctx_cat Γ Δ) :=
-    match Δ with
-    | ctx_nil      => bIn
-    | ctx_snoc Δ _ => inctx_succ (inctx_cat_left Δ bIn)
-    end.
-
-  Fixpoint inctx_cat_right {b : B} {Γ : Ctx B} (Δ : Ctx B) : InCtx b Δ -> InCtx b (ctx_cat Γ Δ) :=
-    match Δ with
-    | ctx_nil      => fun bIn => match nilView bIn with end
-    | ctx_snoc Δ _ =>
-      fun bIn =>
-        match snocView bIn with
-        | snocViewZero => inctx_zero
-        | snocViewSucc bIn => inctx_succ (inctx_cat_right bIn)
-        end
-    end.
-
-  Inductive CatView {Γ Δ} {b : B} : InCtx b (ctx_cat Γ Δ) -> Set :=
-  | isCatLeft  (bIn : InCtx b Γ) : CatView (inctx_cat_left Δ bIn)
-  | isCatRight (bIn : InCtx b Δ) : CatView (inctx_cat_right bIn).
-
-  Definition catView_succ {Γ Δ b b'} (bIn : InCtx b (ctx_cat Γ Δ)) (bInV : CatView bIn) :
-    @CatView Γ (ctx_snoc Δ b') b (inctx_succ bIn) :=
-    match bInV with
-    | isCatLeft bIn => @isCatLeft Γ (@ctx_snoc B Δ b') b bIn
-    | isCatRight bIn => @isCatRight Γ (@ctx_snoc B Δ b') b (@inctx_succ b Δ b' bIn)
-    end.
-
-  Fixpoint catView_index {Γ Δ} {b : B} {struct Δ} :
-    forall (n : nat) (p : ctx_nth_is (ctx_cat Γ Δ) n b),
-      @CatView Γ Δ b (@MkInCtx b (ctx_cat Γ Δ) n p) :=
-    match Δ with
-    | ctx_nil => fun n p => @isCatLeft Γ (@ctx_nil B) b (@MkInCtx b Γ n p)
-    | ctx_snoc Δ0 b0 =>
-      fun n =>
-        match n with
-        | 0 =>
-          fun p =>
-            match
-              p as e in (_ = y)
-              return (@CatView Γ (@ctx_snoc B Δ0 b0) y (@MkInCtx y (@ctx_snoc B (ctx_cat Γ Δ0) b0) 0 e))
-            with
-            | eq_refl => @isCatRight Γ (@ctx_snoc B Δ0 b0) b0 (@inctx_zero b0 Δ0)
-            end
-        | S n => fun p => catView_succ (catView_index n p)
-        end
-    end.
-
-  Definition catView {Γ Δ} {b : B} (bIn : InCtx b (ctx_cat Γ Δ)) : CatView bIn :=
-    @catView_index Γ Δ b (@inctx_at _ _ bIn) (@inctx_valid _ _ bIn).
-
-  (* Custom pattern matching in cases where the context was already refined
-     by a different match, i.e. on environments. *)
-  Definition inctx_case_nil {b : B} {A : Type} (bIn : InCtx b ctx_nil) : A :=
-    match nilView bIn with end.
-  Definition inctx_case_snoc (D : B -> Type) (Γ : Ctx B) (b0 : B) (db0 : D b0)
-    (dΓ: forall b, InCtx b Γ -> D b) (b : B) (bIn: InCtx b (ctx_snoc Γ b0)) : D b :=
-    let (n, e) := bIn in
-    match n return ctx_nth_is (ctx_snoc Γ b0) n b -> D b with
-    | 0 => fun e => match e with eq_refl => db0 end
-    | S n => fun e => dΓ b (MkInCtx n e)
-    end e.
-
-  Definition InCtx_rect (b : B)
-    (P : forall (Γ : Ctx B), InCtx b Γ -> Type)
-    (fzero : forall (Γ : Ctx B), P (ctx_snoc Γ b) inctx_zero)
-    (fsucc : forall (Γ : Ctx B) (b0 : B) (bIn : InCtx b Γ),
-        P Γ bIn -> P (ctx_snoc Γ b0) (inctx_succ bIn)) :
-    forall (Γ : Ctx B) (bIn : InCtx b Γ), P Γ bIn.
-  Proof.
-    induction Γ; cbn.
-    - intro bIn. destruct (nilView bIn).
-    - intros bIn. destruct (snocView bIn).
-      + apply fzero.
-      + now apply fsucc.
-  Defined.
-
-  Definition InCtx_ind (b : B)
-    (P : forall (Γ : Ctx B), InCtx b Γ -> Prop)
-    (fzero : forall (Γ : Ctx B), P (ctx_snoc Γ b) inctx_zero)
-    (fsucc : forall (Γ : Ctx B) (b0 : B) (bIn : InCtx b Γ),
-        P Γ bIn -> P (ctx_snoc Γ b0) (inctx_succ bIn)) :
-    forall (Γ : Ctx B) (bIn : InCtx b Γ), P Γ bIn :=
-    InCtx_rect P fzero fsucc.
-
-  (* Boolean equality of [nat]-fields in [InCtx] implies equality of
-     the other field and the binding-index of [InCtx] *)
-  Lemma inctx_at_exact {Γ : Ctx B} (b1 b2 : B)
-        (b1In : InCtx b1 Γ) (b2In : InCtx b2 Γ) :
-    @inctx_at _ _ b1In = @inctx_at _ _ b2In ->
-    b1 = b2 /\
-    (ctx_nth_is Γ (@inctx_at _ _ b1In) b1 = ctx_nth_is Γ (@inctx_at _ _ b2In) b2).
-  Proof.
-    intros.
-    assert (b1 = b2) as bindings_eq.
-    { generalize dependent b2.
-      induction b1In using InCtx_ind; destruct b2In as [[|n] e];
-      intros; cbn in *; try congruence.
-      apply IHb1In with (MkInCtx n e).
-      cbn; congruence. }
-    split.
-    - exact bindings_eq.
-    - subst. f_equal. assumption.
-  Qed.
-
-  Fixpoint ctx_remove (Γ : Ctx B) {b : B} : InCtx b Γ -> Ctx B :=
-    match Γ with
-    | ctx_nil =>
-      fun '(MkInCtx n e) =>
-        match e with end
-    | ctx_snoc Γ b' =>
-      fun '(MkInCtx n e) =>
-        match n return (ctx_nth_is (ctx_snoc Γ b') n b -> Ctx B)
-        with
-        | 0   => fun _ => Γ
-        | S n => fun e  => ctx_snoc (@ctx_remove Γ b (MkInCtx n e)) b'
-        end e
-    end.
-  Arguments ctx_remove _ [_] _.
-
-  Fixpoint shift_index {b x} {Σ : Ctx B} {struct Σ} :
-    forall
-      (bn xn : nat) (bp : ctx_nth_is Σ bn b)
-      (xp : ctx_nth_is (ctx_remove Σ {| inctx_valid := bp |}) xn x),
-      InCtx x Σ :=
-    match Σ with
-    | ctx_nil => fun _ _ (bp : ctx_nth_is ctx_nil _ _) => match bp with end
-    | ctx_snoc Σ b =>
-      fun bn xn =>
-        match bn , xn with
-        | O    , xn   => fun bp xp => inctx_succ (MkInCtx xn xp)
-        | S bn , O    => fun bp xp => MkInCtx (Γ := ctx_snoc Σ b) O xp
-        | S bn , S xn => fun bp xp => inctx_succ (shift_index bn xn bp xp)
-        end
-    end.
-
-  Definition shift_var {b x} {Σ : Ctx B} (bIn : InCtx b Σ) (xIn : InCtx x (ctx_remove Σ bIn)) : InCtx x Σ :=
-    shift_index (inctx_at bIn) (inctx_at xIn) (inctx_valid bIn) (inctx_valid xIn).
-
-  (* Most explicit type-signatures given below are only necessary for Coq 8.9
-     and can be cleaned up for later versions. *)
-  Fixpoint occurs_check_index {Σ} {x y : B} (m n : nat) {struct Σ} :
-    forall (p : ctx_nth_is Σ m x) (q : ctx_nth_is Σ n y),
-      (x = y) + (InCtx y (ctx_remove _ {| inctx_at := m; inctx_valid := p |})) :=
-    match Σ with
-    | ctx_nil => fun _ (q : ctx_nth_is ctx_nil n y) => match q with end
-    | ctx_snoc Σ b =>
-      match m , n with
-      | 0   , 0   => fun (p : ctx_nth_is (ctx_snoc Σ b) 0 x) q =>
-                       inl (eq_trans (eq_sym p) q)
-      | 0   , S n => fun p (q : ctx_nth_is (ctx_snoc Σ b) (S n) y) =>
-                       inr (@MkInCtx _ (ctx_remove _ (@MkInCtx _ (ctx_snoc Σ b) 0 p)) n q)
-      | S m , 0   => fun _ (q : ctx_nth_is (ctx_snoc Σ b) 0 y) =>
-                       inr (@MkInCtx _ (ctx_snoc (ctx_remove Σ _) b) 0 q)
-      | S m , S n => fun p q => base.sum_map id inctx_succ (occurs_check_index m n p q)
-      end
-    end.
-
-  Definition occurs_check_var {Σ} {x y : B} (xIn : InCtx x Σ) (yIn : InCtx y Σ) : (x = y) + (InCtx y (ctx_remove Σ xIn)) :=
-    occurs_check_index (inctx_at xIn) (inctx_at yIn) (inctx_valid xIn) (inctx_valid yIn).
-
-  Inductive OccursCheckView {Σ} {x : B} (xIn : InCtx x Σ) : forall y, InCtx y Σ -> Set :=
-  | Same : OccursCheckView xIn xIn
-  | Diff {y} (yIn : InCtx y (ctx_remove Σ xIn)) : OccursCheckView xIn (shift_var xIn yIn).
-
-  Definition occurs_check_view_step {Σ} {b x y: B} (xIn : InCtx x Σ) (yIn : InCtx y Σ) :
-    OccursCheckView xIn yIn ->
-    OccursCheckView (Σ := ctx_snoc Σ b) (inctx_succ xIn) (inctx_succ yIn) :=
-    fun v =>
-    match v with
-    | Same _     => Same (inctx_succ xIn)
-    | Diff _ yIn => Diff (inctx_succ xIn) (inctx_succ yIn)
-    end.
-
-  Fixpoint occurs_check_view_index {Σ} {x y: B} {m n : nat} {struct Σ} :
-    forall (p : ctx_nth_is Σ m x) (q : ctx_nth_is Σ n y),
-      OccursCheckView
-        {| inctx_at := m; inctx_valid := p |}
-        {| inctx_at := n; inctx_valid := q |} :=
-    match Σ with
-    | ctx_nil => fun _ (q : ctx_nth_is ctx_nil n y) => match q with end
-    | ctx_snoc Σ b =>
-      match m , n with
-      | 0   , 0   => fun (p : ctx_nth_is (ctx_snoc Σ b) 0 x) q =>
-               match p , q with
-               | eq_refl , eq_refl =>
-                 Same (@MkInCtx b (@ctx_snoc B Σ b) 0 eq_refl)
-               end
-      | 0   , S n => fun p (q : ctx_nth_is (ctx_snoc Σ b) (S n) y) =>
-                       Diff
-                         (@MkInCtx x (@ctx_snoc B Σ b) 0 p)
-                         (@MkInCtx y Σ n q)
-      | S m , 0   => fun p (q : ctx_nth_is (ctx_snoc Σ b) 0 y) =>
-                       Diff
-                         (@MkInCtx x (@ctx_snoc B Σ b) (S m) p)
-                         (@MkInCtx _ (ctx_snoc (ctx_remove Σ _) b) 0 q)
-      | S m , S n => fun p q =>
-                       occurs_check_view_step
-                         (@occurs_check_view_index Σ x y m n p q)
-      end
-    end.
-
-  Definition occurs_check_view {Σ} {x y: B} (xIn : InCtx x Σ) (yIn : InCtx y Σ) : OccursCheckView xIn yIn :=
-    occurs_check_view_index (inctx_valid xIn) (inctx_valid yIn).
-
-  Lemma occurs_check_var_spec {Σ} {x y : B} (xIn : InCtx x Σ) (yIn : InCtx y Σ) :
-    match occurs_check_var xIn yIn with
-    | inl e    => eq_rect x (fun z => InCtx z Σ) xIn y e = yIn
-    | inr yIn' => yIn = shift_var xIn yIn' /\ inctx_at xIn <> inctx_at yIn
-    end%type.
-  Proof.
-    unfold occurs_check_var, shift_var; destruct yIn as [n q]; revert n q.
-    induction xIn using InCtx_ind; intros n q.
-    - destruct n.
-      + now destruct q.
-      + split. reflexivity. cbn. intuition.
-    - destruct n; cbn.
-      + split. reflexivity. intuition.
-      + specialize (IHxIn n q); revert IHxIn; cbn.
-        destruct (occurs_check_index (inctx_at xIn) n (inctx_valid xIn) q).
-        * destruct e; cbn. now intros ->.
-        * destruct xIn as [m p]; cbn. intros [<- ?]. intuition.
-  Qed.
-
-  Lemma occurs_check_var_refl {Σ x} (xIn : InCtx x Σ) :
-    occurs_check_var xIn xIn = inl eq_refl.
-  Proof.
-    unfold occurs_check_var.
-    induction xIn using InCtx_ind.
-    - reflexivity.
-    - cbn; now rewrite IHxIn.
-  Qed.
-
-  Lemma occurs_check_shift_var {x y} {Σ : Ctx B} (xIn : InCtx x Σ) (yIn : InCtx y (ctx_remove Σ xIn)) :
-    occurs_check_var xIn (shift_var xIn yIn) = inr yIn.
-  Proof.
-    unfold occurs_check_var, shift_var. destruct yIn as [m p]. cbn.
-    revert m p.
-    induction xIn using InCtx_ind.
-    - reflexivity.
-    - intros [|m]; cbn.
-      + reflexivity.
-      + intros p.
-        now rewrite (IHxIn m p).
-  Qed.
-
-  Fixpoint ctx_forallb (Γ : Ctx B) : (forall b, InCtx b Γ -> bool) -> bool :=
-    match Γ with
-    | ctx_nil      => fun _ => true
-    | ctx_snoc Γ b => fun p => p b inctx_zero && ctx_forallb (fun b bIn => p b (inctx_succ bIn))
-    end.
-
-  Fixpoint flip_remove_index {Γ : Ctx B} {y x} (n m : nat) {struct Γ} :
-    forall
-      (q : ctx_nth_is Γ n y)
-      (p : ctx_nth_is (ctx_remove Γ {| inctx_at := n; inctx_valid := q |}) m x),
-      InCtx y (ctx_remove Γ (shift_index n m q p)) :=
-   match Γ with
-   | ctx_nil => fun q => match q with end
-   | ctx_snoc Γ b =>
-       match n with
-       | 0 =>
-         fun q p =>
-           @MkInCtx y (ctx_remove (ctx_snoc Γ b) (shift_index 0 m q p)) 0 q
-       | S n =>
-         fun q =>
-           match m with
-           | 0 => fun _ => @MkInCtx y Γ n q
-           | S m => fun p => inctx_succ (flip_remove_index n m q p)
-           end
-       end
-   end.
-
-  (* Calculates x ∈ Γ - y => y ∈ Γ - x *)
-  Definition flip_remove {Γ : Ctx B} {y x : B} (yIn : InCtx y Γ) (xIn : InCtx x (@ctx_remove Γ y yIn)) :
-    InCtx y (@ctx_remove Γ x (@shift_var y x Γ yIn xIn)) :=
-    flip_remove_index (inctx_at yIn) (inctx_at xIn) (inctx_valid yIn) (inctx_valid xIn).
-
-  (* Σ - y - x = Σ - x - y *)
-  Lemma swap_remove {Γ : Ctx B} {y x} (yIn : InCtx y Γ) (xIn : InCtx x (ctx_remove Γ yIn)) :
-    ctx_remove (ctx_remove Γ yIn) xIn =
-    ctx_remove (ctx_remove Γ (shift_var yIn xIn)) (flip_remove yIn xIn).
-  Proof.
-    destruct yIn as [n q], xIn as [m p]. cbn in *.
-    unfold shift_var. cbn.
-    revert n q m p.
-    induction Γ; intros n q m p.
-    destruct q.
-    destruct n; cbn in q.
-    - reflexivity.
-    - destruct m; cbn in p.
-      + reflexivity.
-      + cbn in *. f_equal. apply IHΓ.
-  Defined.
-
-End WithBinding.
-Arguments InCtx_ind [B b] _ _ _ [_].
-Arguments ctx_forallb [B] Γ p.
-
-Section WithAB.
-  Context {A B : Set} (f : A -> B).
-
-  Fixpoint ctx_map (Γ : Ctx A) : Ctx B :=
-    match Γ with
-    | ctx_nil      => ctx_nil
-    | ctx_snoc Γ a => ctx_snoc (ctx_map Γ) (f a)
-    end.
-
-  Fixpoint inctx_map {a : A} {Γ : Ctx A} {struct Γ} : InCtx a Γ -> InCtx (f a) (ctx_map Γ) :=
-   match Γ return InCtx a Γ -> InCtx (f a) (ctx_map Γ) with
-   | ctx_nil => inctx_case_nil
-   | ctx_snoc Γ b =>
-     fun aInΓb  =>
-       match inctx_at aInΓb as n return ctx_nth_is (ctx_snoc Γ b) n a -> _ with
-       | 0   => fun p => @MkInCtx _ _ (ctx_snoc _ _) 0 (f_equal f p)
-       | S n => fun p => inctx_succ (inctx_map {| inctx_at := n; inctx_valid := p |})
-       end (inctx_valid aInΓb)
-   end.
-
-End WithAB.
+Local Set Implicit Arguments.
 
 Module Binding.
 
@@ -577,113 +61,647 @@ Module Binding.
 
 End Binding.
 Export Binding.
-Notation NCtx N T := (Ctx (Binding N T)).
 
-Module CtxNotations.
+Module ctx.
 
-  (* DEPRECATED *)
-  (* NB: ∶ ≠ : *)
-  (*    To typeset the next notation, use \: *)
-  Notation "x ∶ τ" := (MkB x τ) (only parsing) : ctx_scope.
-  Notation "x :: τ" := (MkB x τ) (only parsing) : ctx_scope.
-  Notation "N ∷ T" := (Binding N T) : type_scope.
-  Notation "x ∷ t" := (MkB x t) : ctx_scope.
+  (* Type of contexts. This is a list of bindings of type B. This type and
+     subsequent types use the common notation of snoc lists. *)
+  Inductive Ctx (B : Set) : Set :=
+  | nil
+  | snoc (Γ : Ctx B) (b : B).
 
-  Notation "'ε'" := ctx_nil : ctx_scope.
-  Infix "▻" := ctx_snoc : ctx_scope.
-  Notation "Γ1 ▻▻ Γ2" := (ctx_cat Γ1%ctx Γ2%ctx) : ctx_scope.
-  Notation "b ∈ Γ" := (InCtx b%ctx Γ%ctx) : type_scope.
+  Section TransparentObligations.
+    Local Set Transparent Obligations.
+    Derive NoConfusion for Ctx.
+  End TransparentObligations.
 
-  Notation "[ x ]" := (ctx_snoc ctx_nil x)  : ctx_scope.
-  Notation "[ x , .. , z ]" := (ctx_snoc .. (ctx_snoc ctx_nil x) .. z) : ctx_scope.
-  Notation "Γ - x" := (@ctx_remove _ Γ x _) : ctx_scope.
+  Arguments nil {_}.
+  Arguments snoc {_} _%ctx _%ctx.
 
-End CtxNotations.
+  Section WithBinding.
+    Context {B : Set}.
 
-Open Scope ctx_scope.
-Import CtxNotations.
+    Global Instance eq_dec_ctx (eqB : EqDec B) : EqDec (Ctx B) :=
+      fix eq_dec_ctx (Γ Δ : Ctx B) {struct Γ} : dec_eq Γ Δ :=
+        match Γ , Δ with
+        | nil      , nil      => left eq_refl
+        | snoc Γ b , snoc Δ c => f_equal2_dec snoc noConfusion_inv
+                                   (eq_dec_ctx Γ Δ) (eq_dec b c)
+        | _        , _        => right noConfusion_inv
+        end.
 
-Section Resolution.
+    Fixpoint lookup (Γ : Ctx B) (n : nat) : option B :=
+      match Γ , n with
+      | snoc _ b , O   => Some b
+      | snoc Γ _ , S n => lookup Γ n
+      | _        , _   => None
+      end.
 
-  Context {Name : Set} {Name_eqdec : EqDec Name} {D : Set}.
+    (* Concatenation of two contexts. *)
+    Fixpoint cat (Γ1 Γ2 : Ctx B) {struct Γ2} : Ctx B :=
+      match Γ2 with
+      | nil       => Γ1
+      | snoc Γ2 τ => snoc (cat Γ1 Γ2) τ
+      end.
 
-  Fixpoint ctx_resolve (Γ : NCtx Name D) (x : Name) {struct Γ} : option D :=
-    match Γ with
-    | ε       => None
-    | Γ ▻ y∷d => if Name_eqdec x y then Some d else ctx_resolve Γ x
-    end.
+    (* This is a predicate that that encodes that the de Bruijn index n points
+       to the binding b in Γ. *)
+    Fixpoint nth_is (Γ : Ctx B) (n : nat) (b : B) {struct Γ} : Prop :=
+      match Γ , n with
+      | snoc _ x , O   => x = b
+      | snoc Γ _ , S n => nth_is Γ n b
+      | _        , _   => False
+      end.
 
-  Fixpoint mk_inctx (Γ : NCtx Name D) (x : Name) {struct Γ} :
-    let m := ctx_resolve Γ x in forall (p : IsSome m), x∷fromSome m p ∈ Γ :=
-    match Γ with
-    | ε => fun p => match p with end
-    | Γ ▻ y∷d =>
-      match Name_eqdec x y as s return
-        (forall p, (x∷fromSome (if s then Some d else ctx_resolve Γ x) p) ∈ Γ ▻ y∷d)
+    Lemma nth_is_right_exact {Γ : Ctx B} (n : nat) (b1 b2 : B) :
+      nth_is Γ n b1 -> nth_is Γ n b2 -> b1 = b2.
+    Proof.
+      revert n.
+      induction Γ.
+      - intros ? [].
+      - cbn in *.
+        destruct n. intros e1 e2.
+        refine (eq_trans _ e2).
+        apply eq_sym. auto.
+        apply IHΓ.
+    Qed.
+
+    Section WithUIP.
+
+      Context {UIP_B : UIP B}.
+
+      Fixpoint proof_irrelevance_nth_is {Γ} (n : nat) (b : B) {struct Γ} :
+        forall (p q : nth_is Γ n b), p = q :=
+        match Γ with
+        | nil       => fun p q => match q with end
+        | snoc Γ b' => match n with
+                       | 0   => uip
+                       | S n => proof_irrelevance_nth_is n b
+                       end
+        end.
+
+      Global Instance eqdec_ctx_nth {Γ n b} : EqDec (nth_is Γ n b).
+      Proof. intros p q. left. apply proof_irrelevance_nth_is. Defined.
+
+      Lemma proof_irrelevance_nth_is_refl {Γ} (n : nat) (b : B) (p : nth_is Γ n b) :
+        proof_irrelevance_nth_is n b p p = eq_refl.
+      Proof. apply uip. Qed.
+
+    End WithUIP.
+
+    Section In.
+      (* Set locally only for the definition of In. *)
+      Local Set Primitive Projections.
+
+       (* InCtx represents context containment proofs. This is essentially a
+          well-typed de Bruijn index, i.e. a de Bruijn index with a proof that it
+          resolves to the binding b. This record type is defined using primitive
+          projections to get eta-conversion definitionally. *)
+      Class In (b : B) (Γ : Ctx B) : Set :=
+        MkIn
+          { in_at: nat;
+            in_valid: nth_is Γ in_at b
+          }.
+
+      Global Arguments MkIn [_ _] _ _.
+      Global Arguments in_at [_ _] _.
+      Global Arguments in_valid [_ _] _.
+
+      Global Program Instance NoConfusionPackage_In {uip_B : UIP B} {b Γ} : NoConfusionPackage (In b Γ) :=
+         {| NoConfusion xIn yIn := NoConfusion (in_at xIn) (in_at yIn);
+            noConfusion xIn yIn (e : NoConfusion (in_at xIn) (in_at yIn)) :=
+              match noConfusion e in _ = y
+                return forall q, xIn = {| in_at := y; in_valid := q |}
+              with
+              | eq_refl => fun q => f_equal (MkIn _) (proof_irrelevance_nth_is _ _ (in_valid xIn) q)
+              end (in_valid yIn);
+            noConfusion_inv (xIn yIn : In b Γ) (e : xIn = yIn) :=
+              noConfusion_inv (f_equal (@in_at b Γ) e);
+         |}.
+      Next Obligation.
+        intros ? ? ? [m p] [n q] e. cbn [in_at] in *.
+        change (NoConfusion _ _) with (NoConfusion m n) in e.
+        destruct (noConfusion e) eqn:?. cbn.
+        destruct (proof_irrelevance_nth_is m b p q). cbn.
+        destruct m.
+        - destruct e. reflexivity.
+        - apply uip.
+      Qed.
+      Next Obligation.
+        intros ? ? ? [m p] [n q] e; intros.
+        destruct e.
+        destruct Γ; cbn in *. contradiction.
+        destruct m, n.
+        - destruct p. cbn. now rewrite EqDec.uip_refl_refl.
+        - destruct p. cbn. now rewrite EqDec.uip_refl_refl.
+        - cbn. rewrite proof_irrelevance_nth_is_refl. reflexivity.
+        - cbn. rewrite proof_irrelevance_nth_is_refl. reflexivity.
+      Qed.
+
+    End In.
+
+    (* Two proofs of context containment are equal of the deBruijn indices are equal *)
+    Definition In_eqb {Γ} {b1 b2 : B} (b1inΓ : In b1 Γ) (b2inΓ : In b2 Γ) : bool :=
+      Nat.eqb (in_at b1inΓ) (in_at b2inΓ).
+
+    Lemma In_eqb_spec `{UIP B} {Γ} {b1 b2 : B} (b1inΓ : In b1 Γ) (b2inΓ : In b2 Γ) :
+      reflect
+        (existT _ b1inΓ = existT _ b2inΓ :> sigT (fun b => In b Γ))
+        (In_eqb b1inΓ b2inΓ).
+    Proof.
+      destruct b1inΓ as [m p], b2inΓ as [n q]; cbn.
+      destruct (NPeano.Nat.eqb_spec m n); constructor.
+      - subst. pose proof (nth_is_right_exact _ _ _ p q). subst.
+        f_equal. f_equal. apply proof_irrelevance_nth_is.
+      - intros e. depelim e. destruct n, m; cbn in H0; congruence.
+    Qed.
+
+    (* These are *constructors* for In. *)
+    Definition in_zero {b : B} {Γ : Ctx B} : In b (snoc Γ b) :=
+      @MkIn _ (snoc Γ b) 0 eq_refl.
+    Definition in_succ {b : B} {Γ : Ctx B} {b' : B} (bIn : In b Γ) :
+      In b (snoc Γ b') :=
+      @MkIn _ (snoc Γ b') (S (in_at bIn)) (in_valid bIn).
+
+    Inductive NilView {b : B} (i : In b nil) : Set :=.
+
+    Definition nilView {b : B} (i : In b nil) : NilView i :=
+      match in_valid i with end.
+
+    Inductive SnocView (Γ : Ctx B) {b' : B} : forall b, In b (snoc Γ b') -> Set :=
+    | snocViewZero                  : SnocView in_zero
+    | snocViewSucc {b} (i : In b Γ) : SnocView (in_succ i).
+    Global Arguments snocViewZero {_ _}.
+
+    Definition snocView {Γ} {b b' : B} (i : In b (snoc Γ b')) :
+      @SnocView Γ b' b i :=
+      match in_at i as n return forall p, SnocView (MkIn n p)
       with
-      | left e => fun _ => match e with eq_refl => inctx_zero end
-      | right _ => fun p => inctx_succ (mk_inctx Γ x p)
-      end
-    end.
+      | O   => fun p => match p with eq_refl => snocViewZero end
+      | S n => fun p => snocViewSucc (MkIn n p)
+      end (in_valid i).
 
-  Fixpoint ctx_names (Γ : NCtx Name D) : list Name :=
-    match Γ with
-    | ε         => nil
-    | Γ ▻ (y∷_) => cons y (ctx_names Γ)
-    end.
+    Inductive InView {b : B} : forall Γ, In b Γ -> Set :=
+    | inctxViewZero {Γ}                 : @InView b (snoc Γ b) in_zero
+    | inctxViewSucc {Γ b'} (i : In b Γ) : @InView b (snoc Γ b') (in_succ i).
 
-End Resolution.
+    Definition inView {b Γ} (bIn : In b Γ) : InView bIn.
+    Proof.
+      destruct Γ.
+      - destruct (nilView bIn).
+      - destruct (snocView bIn); constructor.
+    Defined.
 
-Module NameResolution.
+    Fixpoint in_cat_left {b : B} {Γ : Ctx B} (Δ : Ctx B) (bIn : In b Γ) : In b (cat Γ Δ) :=
+      match Δ with
+      | nil      => bIn
+      | snoc Δ _ => in_succ (in_cat_left Δ bIn)
+      end.
 
-  (* Hook the reflective procedure for name resolution into the typeclass
-     resolution mechanism. *)
-  Hint Extern 10 (?x∷_ ∈ ?Γ) =>
-    let xInΓ := eval compute in (mk_inctx Γ x tt) in
-      exact xInΓ : typeclass_instances.
+    Fixpoint in_cat_right {b : B} {Γ : Ctx B} (Δ : Ctx B) : In b Δ -> In b (cat Γ Δ) :=
+      match Δ with
+      | nil      => fun bIn => match nilView bIn with end
+      | snoc _ _ =>
+        fun bIn =>
+          match snocView bIn with
+          | snocViewZero => in_zero
+          | snocViewSucc bIn => in_succ (in_cat_right bIn)
+          end
+      end.
 
-End NameResolution.
+    Inductive CatView {Γ Δ} {b : B} : In b (cat Γ Δ) -> Set :=
+    | isCatLeft  (bIn : In b Γ) : CatView (in_cat_left Δ bIn)
+    | isCatRight (bIn : In b Δ) : CatView (in_cat_right bIn).
 
-Section FreshName.
+    Definition catView_succ {Γ Δ b b'} (bIn : In b (cat Γ Δ)) (bInV : CatView bIn) :
+      @CatView Γ (snoc Δ b') b (in_succ bIn) :=
+      match bInV with
+      | isCatLeft bIn => @isCatLeft Γ (@snoc B Δ b') b bIn
+      | isCatRight bIn => @isCatRight Γ (@snoc B Δ b') b (@in_succ b Δ b' bIn)
+      end.
 
-  Local Open Scope string_scope.
+    Fixpoint catView_index {Γ Δ} {b : B} {struct Δ} :
+      forall (n : nat) (p : nth_is (cat Γ Δ) n b),
+        @CatView Γ Δ b (@MkIn b (cat Γ Δ) n p) :=
+      match Δ with
+      | nil => fun n p => @isCatLeft Γ (@nil B) b (@MkIn b Γ n p)
+      | snoc Δ0 b0 =>
+        fun n =>
+          match n with
+          | 0 =>
+            fun p =>
+              match
+                p as e in (_ = y)
+                return (@CatView Γ (@snoc B Δ0 b0) y (@MkIn y (@snoc B (cat Γ Δ0) b0) 0 e))
+              with
+              | eq_refl => @isCatRight Γ (@snoc B Δ0 b0) b0 (@in_zero b0 Δ0)
+              end
+          | S n => fun p => catView_succ (catView_index n p)
+          end
+      end.
 
-  Fixpoint split_at_dot' {R} (x : string) (k : string -> string -> R) {struct x} : R :=
-    match x with
-    | ""           => k "" ""
-    | String "." x => k "" x
-    | String a x   => split_at_dot' x (fun pre => k (String a pre))
-    end.
+    Definition catView {Γ Δ} {b : B} (bIn : In b (cat Γ Δ)) : CatView bIn :=
+      @catView_index Γ Δ b (@in_at _ _ bIn) (@in_valid _ _ bIn).
 
-  Definition split_at_dot (x : string) : (string * string) :=
-    split_at_dot' x pair.
+    (* Custom pattern matching in cases where the context was already refined
+       by a different match, i.e. on environments. *)
+    Definition in_case_nil {b : B} {A : Type} (bIn : In b nil) : A :=
+      match nilView bIn with end.
+    Definition in_case_snoc (D : B -> Type) (Γ : Ctx B) (b0 : B) (db0 : D b0)
+      (dΓ: forall b, In b Γ -> D b) (b : B) (bIn: In b (snoc Γ b0)) : D b :=
+      let (n, e) := bIn in
+      match n return nth_is (snoc Γ b0) n b -> D b with
+      | 0 => fun e => match e with eq_refl => db0 end
+      | S n => fun e => dΓ b (MkIn n e)
+      end e.
 
-  Definition parse_number (x : string) : N :=
-    match NilEmpty.uint_of_string x with
-    | Some n => N.of_uint n
-    | None   => 0%N
-    end.
+    Definition In_rect (b : B)
+      (P : forall (Γ : Ctx B), In b Γ -> Type)
+      (fzero : forall (Γ : Ctx B), P (snoc Γ b) in_zero)
+      (fsucc : forall (Γ : Ctx B) (b0 : B) (bIn : In b Γ),
+          P Γ bIn -> P (snoc Γ b0) (in_succ bIn)) :
+      forall (Γ : Ctx B) (bIn : In b Γ), P Γ bIn.
+    Proof.
+      induction Γ; cbn.
+      - intro bIn. destruct (nilView bIn).
+      - intros bIn. destruct (snocView bIn).
+        + apply fzero.
+        + now apply fsucc.
+    Defined.
+    Global Arguments In_rect [_] _.
 
-  Definition unparse_number (x : N) : string :=
-    NilEmpty.string_of_uint (N.to_uint x).
+    Definition In_ind (b : B)
+      (P : forall (Γ : Ctx B), In b Γ -> Prop)
+      (fzero : forall (Γ : Ctx B), P (snoc Γ b) in_zero)
+      (fsucc : forall (Γ : Ctx B) (b0 : B) (bIn : In b Γ),
+          P Γ bIn -> P (snoc Γ b0) (in_succ bIn)) :
+      forall (Γ : Ctx B) (bIn : In b Γ), P Γ bIn :=
+      In_rect P fzero fsucc.
+    Global Arguments In_ind [_] _.
 
-  Definition max_with_base (base : string) (xs : list string) : N :=
-    List.fold_left
-      (fun o x =>
-         match split_at_dot x with
-           (pre,suf) => if pre =? base
-                        then N.max o (parse_number suf)
-                        else o
-         end)
-      xs 0%N.
+    (* Boolean equality of [nat]-fields in [In] implies equality of
+       the other field and the binding-index of [In] *)
+    Lemma in_at_exact {Γ : Ctx B} (b1 b2 : B)
+          (b1In : In b1 Γ) (b2In : In b2 Γ) :
+      @in_at _ _ b1In = @in_at _ _ b2In ->
+      b1 = b2 /\
+      (nth_is Γ (@in_at _ _ b1In) b1 = nth_is Γ (@in_at _ _ b2In) b2).
+    Proof.
+      intros.
+      assert (b1 = b2) as bindings_eq.
+      { generalize dependent b2.
+        induction b1In using In_ind; destruct b2In as [[|n] e];
+        intros; cbn in *; try congruence.
+        apply IHb1In with (MkIn n e).
+        cbn; congruence. }
+      split.
+      - exact bindings_eq.
+      - subst. f_equal. assumption.
+    Qed.
 
-  Definition fresh {T : Set} (xs : NCtx string T) (x : option string) : string :=
-    let xs := ctx_names xs in
-    let x := match x with Some x => x | None => "x" end in
-    if List.find (String.eqb x) xs
-    then let base := fst (split_at_dot x) in
-         let n    := N.succ (max_with_base base xs) in
-         String.append base (String "."%char (unparse_number n))
-    else x.
+    Fixpoint remove (Γ : Ctx B) {b : B} : In b Γ -> Ctx B :=
+      match Γ with
+      | nil =>
+        fun '(MkIn n e) =>
+          match e with end
+      | snoc Γ b' =>
+        fun '(MkIn n e) =>
+          match n return (nth_is (snoc Γ b') n b -> Ctx B)
+          with
+          | 0   => fun _ => Γ
+          | S n => fun e  => snoc (@remove Γ b (MkIn n e)) b'
+          end e
+      end.
+    Arguments remove _ [_] _.
 
-End FreshName.
+    Fixpoint shift_index {b x} {Σ : Ctx B} {struct Σ} :
+      forall
+        (bn xn : nat) (bp : nth_is Σ bn b)
+        (xp : nth_is (remove Σ {| in_valid := bp |}) xn x),
+        In x Σ :=
+      match Σ with
+      | nil => fun _ _ (bp : nth_is nil _ _) => match bp with end
+      | snoc Σ b =>
+        fun bn xn =>
+          match bn , xn with
+          | O    , xn   => fun bp xp => in_succ (MkIn xn xp)
+          | S bn , O    => fun bp xp => MkIn (Γ := snoc Σ b) O xp
+          | S bn , S xn => fun bp xp => in_succ (shift_index bn xn bp xp)
+          end
+      end.
+
+    Definition shift_var {b x} {Σ : Ctx B} (bIn : In b Σ) (xIn : In x (remove Σ bIn)) : In x Σ :=
+      shift_index (in_at bIn) (in_at xIn) (in_valid bIn) (in_valid xIn).
+
+    (* Most explicit type-signatures given below are only necessary for Coq 8.9
+       and can be cleaned up for later versions. *)
+    Fixpoint occurs_check_index {Σ} {x y : B} (m n : nat) {struct Σ} :
+      forall (p : nth_is Σ m x) (q : nth_is Σ n y),
+        (x = y) + (In y (remove _ {| in_at := m; in_valid := p |})) :=
+      match Σ with
+      | nil => fun _ (q : nth_is nil n y) => match q with end
+      | snoc Σ b =>
+        match m , n with
+        | 0   , 0   => fun (p : nth_is (snoc Σ b) 0 x) q =>
+                         inl (eq_trans (eq_sym p) q)
+        | 0   , S n => fun p (q : nth_is (snoc Σ b) (S n) y) =>
+                         inr (@MkIn _ (remove _ (@MkIn _ (snoc Σ b) 0 p)) n q)
+        | S m , 0   => fun _ (q : nth_is (snoc Σ b) 0 y) =>
+                         inr (@MkIn _ (snoc (remove Σ _) b) 0 q)
+        | S m , S n => fun p q => base.sum_map id in_succ (occurs_check_index m n p q)
+        end
+      end.
+
+    Definition occurs_check_var {Σ} {x y : B} (xIn : In x Σ) (yIn : In y Σ) : (x = y) + (In y (remove Σ xIn)) :=
+      occurs_check_index (in_at xIn) (in_at yIn) (in_valid xIn) (in_valid yIn).
+
+    Inductive OccursCheckView {Σ} {x : B} (xIn : In x Σ) : forall y, In y Σ -> Set :=
+    | Same : OccursCheckView xIn xIn
+    | Diff {y} (yIn : In y (remove Σ xIn)) : OccursCheckView xIn (shift_var xIn yIn).
+
+    Definition occurs_check_view_step {Σ} {b x y: B} (xIn : In x Σ) (yIn : In y Σ) :
+      OccursCheckView xIn yIn ->
+      OccursCheckView (Σ := snoc Σ b) (in_succ xIn) (in_succ yIn) :=
+      fun v =>
+      match v with
+      | Same _     => Same (in_succ xIn)
+      | Diff _ yIn => Diff (in_succ xIn) (in_succ yIn)
+      end.
+
+    Fixpoint occurs_check_view_index {Σ} {x y: B} {m n : nat} {struct Σ} :
+      forall (p : nth_is Σ m x) (q : nth_is Σ n y),
+        OccursCheckView
+          {| in_at := m; in_valid := p |}
+          {| in_at := n; in_valid := q |} :=
+      match Σ with
+      | nil => fun _ (q : nth_is nil n y) => match q with end
+      | snoc Σ b =>
+        match m , n with
+        | 0   , 0   => fun (p : nth_is (snoc Σ b) 0 x) q =>
+                         match p , q with
+                         | eq_refl , eq_refl =>
+                             Same (@MkIn b (@snoc B Σ b) 0 eq_refl)
+                         end
+        | 0   , S n => fun p (q : nth_is (snoc Σ b) (S n) y) =>
+                         Diff
+                           (@MkIn x (@snoc B Σ b) 0 p)
+                           (@MkIn y Σ n q)
+        | S m , 0   => fun p (q : nth_is (snoc Σ b) 0 y) =>
+                         Diff
+                           (@MkIn x (@snoc B Σ b) (S m) p)
+                           (@MkIn _ (snoc (remove Σ _) b) 0 q)
+        | S m , S n => fun p q =>
+                         occurs_check_view_step
+                           (@occurs_check_view_index Σ x y m n p q)
+        end
+      end.
+
+    Definition occurs_check_view {Σ} {x y: B} (xIn : In x Σ) (yIn : In y Σ) : OccursCheckView xIn yIn :=
+      occurs_check_view_index (in_valid xIn) (in_valid yIn).
+
+    Lemma occurs_check_var_spec {Σ} {x y : B} (xIn : In x Σ) (yIn : In y Σ) :
+      match occurs_check_var xIn yIn with
+      | inl e    => eq_rect x (fun z => In z Σ) xIn y e = yIn
+      | inr yIn' => yIn = shift_var xIn yIn' /\ in_at xIn <> in_at yIn
+      end%type.
+    Proof.
+      unfold occurs_check_var, shift_var; destruct yIn as [n q]; revert n q.
+      induction xIn using In_ind; intros n q.
+      - destruct n.
+        + now destruct q.
+        + split. reflexivity. cbn. intuition.
+      - destruct n; cbn.
+        + split. reflexivity. intuition.
+        + specialize (IHxIn n q); revert IHxIn; cbn.
+          destruct (occurs_check_index (in_at xIn) n (in_valid xIn) q).
+          * destruct e; cbn. now intros ->.
+          * destruct xIn as [m p]; cbn. intros [<- ?]. intuition.
+    Qed.
+
+    Lemma occurs_check_var_refl {Σ x} (xIn : In x Σ) :
+      occurs_check_var xIn xIn = inl eq_refl.
+    Proof.
+      unfold occurs_check_var.
+      induction xIn using In_ind.
+      - reflexivity.
+      - cbn; now rewrite IHxIn.
+    Qed.
+
+    Lemma occurs_check_shift_var {Σ x y} (xIn : In x Σ) (yIn : In y (remove Σ xIn)) :
+      occurs_check_var xIn (shift_var xIn yIn) = inr yIn.
+    Proof.
+      unfold occurs_check_var, shift_var. destruct yIn as [m p]. cbn.
+      revert m p.
+      induction xIn using In_ind.
+      - reflexivity.
+      - intros [|m]; cbn.
+        + reflexivity.
+        + intros p.
+          now rewrite (IHxIn m p).
+    Qed.
+
+    Local Open Scope lazy_bool_scope.
+
+    Fixpoint forallb (Γ : Ctx B) : (forall b, In b Γ -> bool) -> bool :=
+      match Γ with
+      | nil      => fun _ => true
+      | snoc Γ b => fun p => p b in_zero &&& forallb (fun b bIn => p b (in_succ bIn))
+      end.
+
+    Fixpoint flip_remove_index {Γ : Ctx B} {y x} (n m : nat) {struct Γ} :
+      forall
+        (q : nth_is Γ n y)
+        (p : nth_is (remove Γ {| in_at := n; in_valid := q |}) m x),
+        In y (remove Γ (shift_index n m q p)) :=
+     match Γ with
+     | nil => fun q => match q with end
+     | snoc Γ b =>
+         match n with
+         | 0 =>
+           fun q p =>
+             @MkIn y (remove (snoc Γ b) (shift_index 0 m q p)) 0 q
+         | S n =>
+           fun q =>
+             match m with
+             | 0 => fun _ => @MkIn y Γ n q
+             | S m => fun p => in_succ (flip_remove_index n m q p)
+             end
+         end
+     end.
+
+    (* Calculates x ∈ Γ - y => y ∈ Γ - x *)
+    Definition flip_remove {Γ : Ctx B} {y x : B} (yIn : In y Γ) (xIn : In x (@remove Γ y yIn)) :
+      In y (@remove Γ x (@shift_var y x Γ yIn xIn)) :=
+      flip_remove_index (in_at yIn) (in_at xIn) (in_valid yIn) (in_valid xIn).
+
+    (* Σ - y - x = Σ - x - y *)
+    Lemma swap_remove {Γ : Ctx B} {y x} (yIn : In y Γ) (xIn : In x (remove Γ yIn)) :
+      remove (remove Γ yIn) xIn =
+      remove (remove Γ (shift_var yIn xIn)) (flip_remove yIn xIn).
+    Proof.
+      destruct yIn as [n q], xIn as [m p]. cbn in *.
+      unfold shift_var. cbn.
+      revert n q m p.
+      induction Γ; intros n q m p.
+      destruct q.
+      destruct n; cbn in q.
+      - reflexivity.
+      - destruct m; cbn in p.
+        + reflexivity.
+        + cbn in *. f_equal. apply IHΓ.
+    Defined.
+
+    Lemma remove_in_cat_right {Γ Δ : Ctx B} {b : B} (bIn : In b Δ) :
+      @remove (@cat Γ Δ) b (@in_cat_right b Γ Δ bIn) =
+      @cat Γ (@remove Δ b bIn).
+    Proof.
+      induction bIn using In_rect; cbn.
+      - reflexivity.
+      - f_equal. auto.
+    Defined.
+
+  End WithBinding.
+  Arguments In_rect [B b] _ _ _ [_].
+  Arguments In_ind [B b] _ _ _ [_].
+  Arguments forallb [B] Γ p.
+
+  Section WithAB.
+    Context {A B : Set} (f : A -> B).
+
+    Fixpoint map (Γ : Ctx A) : Ctx B :=
+      match Γ with
+      | nil      => nil
+      | snoc Γ a => snoc (map Γ) (f a)
+      end.
+
+    Fixpoint in_map {a : A} {Γ : Ctx A} {struct Γ} : In a Γ -> In (f a) (map Γ) :=
+     match Γ return In a Γ -> In (f a) (map Γ) with
+     | nil => in_case_nil
+     | snoc Γ b =>
+       fun aInΓb  =>
+         match in_at aInΓb as n return nth_is (snoc Γ b) n a -> _ with
+         | 0   => fun p => @MkIn _ _ (snoc _ _) 0 (f_equal f p)
+         | S n => fun p => in_succ (in_map {| in_at := n; in_valid := p |})
+         end (in_valid aInΓb)
+     end.
+
+  End WithAB.
+
+  Module notations.
+
+    Open Scope ctx_scope.
+
+    (* DEPRECATED *)
+    (* NB: ∶ ≠ : *)
+    (*    To typeset the next notation, use \: *)
+    Notation "x ∶ τ" := (MkB x τ) (only parsing) : ctx_scope.
+    Notation "x :: τ" := (MkB x τ) (only parsing) : ctx_scope.
+    Notation "N ∷ T" := (Binding N T) : type_scope.
+    Notation "x ∷ t" := (MkB x t) : ctx_scope.
+
+    Notation "'ε'" := nil : ctx_scope.
+    Infix "▻" := snoc : ctx_scope.
+    Notation "Γ1 ▻▻ Γ2" := (cat Γ1%ctx Γ2%ctx) : ctx_scope.
+    Notation "b ∈ Γ" := (In b%ctx Γ%ctx) : type_scope.
+
+    Notation "[ x ]" := (snoc nil x)  : ctx_scope.
+    Notation "[ x , .. , z ]" := (snoc .. (snoc nil x) .. z) : ctx_scope.
+    Notation "Γ - x" := (@remove _ Γ x _) : ctx_scope.
+
+  End notations.
+  Import notations.
+
+  Local Notation NCtx N T := (Ctx (Binding N T)).
+
+  Section Resolution.
+
+    Context {Name : Set} {Name_eqdec : EqDec Name} {D : Set}.
+
+    Fixpoint resolve (Γ : NCtx Name D) (x : Name) {struct Γ} : option D :=
+      match Γ with
+      | ε       => None
+      | Γ ▻ y∷d => if Name_eqdec x y then Some d else resolve Γ x
+      end.
+
+    Fixpoint resolve_mk_in (Γ : NCtx Name D) (x : Name) {struct Γ} :
+      let m := resolve Γ x in forall (p : IsSome m), x∷fromSome m p ∈ Γ :=
+      match Γ with
+      | ε => fun p => match p with end
+      | Γ ▻ y∷d =>
+        match Name_eqdec x y as s return
+          (forall p, (x∷fromSome (if s then Some d else resolve Γ x) p) ∈ Γ ▻ y∷d)
+        with
+        | left e => fun _ => match e with eq_refl => in_zero end
+        | right _ => fun p => in_succ (resolve_mk_in Γ x p)
+        end
+      end.
+
+    Fixpoint names (Γ : NCtx Name D) : list Name :=
+      match Γ with
+      | ε       => List.nil
+      | Γ ▻ y∷_ => cons y (names Γ)
+      end.
+
+  End Resolution.
+
+  Module resolution.
+
+    (* Hook the reflective procedure for name resolution into the typeclass
+       resolution mechanism. *)
+    #[export]
+    Hint Extern 10 (?x∷_ ∈ ?Γ) =>
+      let xInΓ := eval compute in (resolve_mk_in Γ x tt) in
+        exact xInΓ : typeclass_instances.
+
+  End resolution.
+
+  Section FreshName.
+
+    Open Scope string_scope.
+
+    Fixpoint split_at_dot' {R} (x : string) (k : string -> string -> R) {struct x} : R :=
+      match x with
+      | ""           => k "" ""
+      | String "." x => k "" x
+      | String a x   => split_at_dot' x (fun pre => k (String a pre))
+      end.
+
+    Definition split_at_dot (x : string) : (string * string) :=
+      split_at_dot' x pair.
+
+    Definition parse_number (x : string) : N :=
+      match NilEmpty.uint_of_string x with
+      | Some n => N.of_uint n
+      | None   => 0%N
+      end.
+
+    Definition unparse_number (x : N) : string :=
+      NilEmpty.string_of_uint (N.to_uint x).
+
+    Definition max_with_base (base : string) (xs : list string) : N :=
+      List.fold_left
+        (fun o x =>
+           match split_at_dot x with
+             (pre,suf) => if pre =? base
+                          then N.max o (parse_number suf)
+                          else o
+           end)
+        xs 0%N.
+
+    Definition fresh {T : Set} (xs : NCtx string T) (x : option string) : string :=
+      let xs := names xs in
+      let x := match x with Some x => x | None => "x" end in
+      if List.find (String.eqb x) xs
+      then let base := fst (split_at_dot x) in
+           let n    := N.succ (max_with_base base xs) in
+           String.append base (String "."%char (unparse_number n))
+      else x.
+
+  End FreshName.
+
+End ctx.
+Import ctx.
+Notation Ctx := ctx.Ctx.
+Notation NCtx N T := (Ctx (Binding N T)).
+Bind Scope ctx_scope with Ctx.
+Bind Scope ctx_scope with NCtx.
