theories/SmallStep/Inversion.v
@@ -36,7 +36,7 @@ From Katamaran Require Import
 
 Set Implicit Arguments.
 
-Import CtxNotations.
+Import ctx.notations.
 Import EnvNotations.
 
 Module Inversion
@@ -268,7 +268,7 @@ Module Inversion
   Qed.
 
   Lemma steps_inversion_block {Γ Δ σ} {γ1 γ3 : RegStore} {μ1 μ3 : Memory} {δ1 δ3 : CStore Γ}
-    {δΔ : CStore Δ} {k : Stm (ctx_cat Γ Δ) σ} {t : Stm Γ σ} (final : Final t)
+    {δΔ : CStore Δ} {k : Stm (Γ ▻▻ Δ) σ} {t : Stm Γ σ} (final : Final t)
     (steps : ⟨ γ1, μ1, δ1, stm_block δΔ k ⟩ --->* ⟨ γ3, μ3, δ3, t ⟩) :
     exists δΔ' k',
       ⟨ γ1, μ1, env_cat δ1 δΔ , k ⟩ --->* ⟨ γ3, μ3, env_cat δ3 δΔ' , k' ⟩ /\ Final k' /\
@@ -351,7 +351,7 @@ Module Inversion
   Qed.
 
   Lemma steps_inversion_ex_block {Γ Δ σ} {γ1 γ3 : RegStore} {μ1 μ3 : Memory} {δ1 δ3 : CStore Γ}
-    {δΔ : CStore Δ} {k : Stm (ctx_cat Γ Δ) σ} {t : Stm Γ σ} (final : Final t)
+    {δΔ : CStore Δ} {k : Stm (Γ ▻▻ Δ) σ} {t : Stm Γ σ} (final : Final t)
     (steps : ⟨ γ1, μ1, δ1, stm_block δΔ k ⟩ --->* ⟨ γ3, μ3, δ3, t ⟩) :
     (exists δΔ' msg,
         ⟨ γ1, μ1, env_cat δ1 δΔ , k ⟩ --->* ⟨ γ3, μ3, env_cat δ3 δΔ' , stm_fail _ msg ⟩ /\
